ebpf/Machregs.v
@@ -182,6 +182,7 @@ Definition two_address_op (op: operation) : bool :=
   | Ocast8signed | Ocast16signed => true
     (* 64 bits *)
   | Ocast32unsigned | Ocast32signed | Olowlong
+  | Ocmp (Ccompl _ | Ccomplu _ | Ccomplimm _ _ | Ccompluimm _ _)
   | Oaddl | Oaddlimm _ | Onegl | Osubl | Osublimm _
   | Omull | Omullimm _ | Odivlu | Omodlu
   | Oandl | Oandlimm _ | Oorl | Oorlimm _
